Relico.lean
@@ -21,6 +21,7 @@ import Relico.Translation.Basic
 import Relico.Correctness.Expression
 import Relico.Correctness.Structural
 import Relico.Correctness.Correspondence
+import Relico.Correctness.Forward
 
 import Relico.Tests.DTRWellFormed
 import Relico.Tests.Translation
@@ -28,3 +29,4 @@ import Relico.Tests.ExpressionCorrectness
 import Relico.Tests.StructuralCorrectness
 import Relico.Tests.SmallStep
 import Relico.Tests.Correspondence
+import Relico.Tests.ForwardSimulation
